Add tactics for fuel, comparison and induction. Able to name with idents instead of strings.

tests/coq/hashmap/Hashmap_Properties.v
@@ -21,6 +21,11 @@ Import ListNotations.
 
 Module Hashmap_Properties.
 
+(*  +-------------+
+    | Definitions |
+    +-------------+
+*)
+
 (* Utilities for the hashmap *)
 
 Definition key_id   := usize.
@@ -28,16 +33,37 @@ Definition hash_id  := usize.
 Definition slot_id  := usize.
 Definition chain_id := usize.
 
-Definition chain_t T := list (usize * T).
+Definition chain_t T := list (key_id * T).
 
-Fixpoint list_t_to_chain {T} (l: List_t T) : chain_t T :=
+Fixpoint to_chain {T} (l: List_t T) : chain_t T :=
     match l with
-    | ListCons n x t => cons (n, x) (list_t_to_chain t)
+    | ListCons n x t => cons (n, x) (to_chain t)
     | ListNil => nil
     end.
 
 Definition get_slots_len {T} (hm: Hash_map_t T) : usize :=
     vec_len (List_t T) hm.(Hash_map_slots).
+
+Definition slots_to_chains {T} (slots: vec (List_t T)) : list (chain_t T) :=
+  List.map to_chain (vec_to_list slots).
+
+Fixpoint get_chain_value {T} (ch: chain_t T) (k: key_id) :
+    option T :=
+  match ch with
+  | [] => None
+  | (k', v) :: t => if (k s= k')
+      then Some v
+      else get_chain_value t k
+  end.
+
+Fixpoint update_chain {T} (ch: chain_t T) (k: key_id) (v: T) :
+    chain_t T :=
+  match ch with
+  | [] => []
+  | (k', v') :: t => if (k s= k')
+      then (k,  v)  :: t
+      else (k', v') :: update_chain t k v
+  end.
 
 (* Hash *)
 
@@ -49,9 +75,9 @@ Definition get_hash_pos {T} (hm: Hash_map_t T) (k: key_id) : result slot_id :=
 
 (* Given hm, i, j: give key-value pair *)
 Definition get_kv {T} (hm: Hash_map_t T) (i: slot_id) (j: chain_id) : result (usize * T) :=
-    let l := vec_to_list hm.(Hash_map_slots) in
+    let l := slots_to_chains hm.(Hash_map_slots) in
     ch <- res_of_opt (nth_error l (usize_to_nat i));
-    let kv := nth_error (list_t_to_chain ch) (usize_to_nat j) in
+    let kv := nth_error ch (usize_to_nat j) in
     res_of_opt kv.
 
 Definition result_prop_bind {T} (x: result T) (p: T -> Prop) : Prop :=
@@ -60,6 +86,46 @@ Definition result_prop_bind {T} (x: result T) (p: T -> Prop) : Prop :=
     | Fail_ OutOfFuel => True
     | Return x => p x
     end.
+
+(* Hashmap length *)
+
+Definition hm_length {T} (hm: Hash_map_t T) : usize :=
+  hm.(Hash_map_num_entries).
+
+Lemma hm_len_success {T} hm :
+  hash_map_len_fwd T hm = Return (hm_length hm).
+Proof.
+reflexivity.
+Qed.
+
+(* Main invariants *)
+
+Notation "x <-- c1 ; c2" := (result_prop_bind c1 (fun x => c2))
+(at level 61, c1 at next level, right associativity).
+
+Definition key_is_in_hash_slot {T} (hm: Hash_map_t T) (i: slot_id) (j: chain_id) : Prop :=
+    kv <-- get_kv hm i j;
+    p  <-- get_hash_pos hm (fst kv);
+    (p = i).
+
+Definition no_key_duplicate {T} (hm: Hash_map_t T) (i: slot_id) (j1 j2: chain_id) (p: j1 <> j2) : Prop :=
+    kv1 <-- get_kv hm i j1;
+    kv2 <-- get_kv hm i j2;
+    (fst kv1 <> fst kv2).
+
+Definition hm_invariants {T} (hm: Hash_map_t T) :=
+    (∀i j, key_is_in_hash_slot hm i j) /\
+    (∀i j1 j2 p, no_key_duplicate hm i j1 j2 p).
+
+(* It may be easier to prove than no_key_duplicate *)
+Definition no_key_duplicate_v2 {T} (hm: Hash_map_t T) : Prop :=
+  let chains := slots_to_chains hm.(Hash_map_slots) in
+  NoDup (map fst (List.concat chains)).
+
+(*  +----------+
+    | Theorems |
+    +----------+
+*)
 
 (* The test from Hashmap_funs.v *)
 
@@ -72,9 +138,6 @@ Qed.
 
 (* Allocate slots *)
 
-Definition slots_to_chains {T}(slots: vec (List_t T)) : list (chain_t T) :=
-    List.map list_t_to_chain (vec_to_list slots).
-
 Lemma hm_allocate_slots_shape (T: Type) (n: usize) (v: vec (List_t T)) (fuel: nat) :
     vec_length v + to_Z n <= usize_max ->
     match hash_map_allocate_slots_fwd T fuel v n with
@@ -85,62 +148,64 @@ Lemma hm_allocate_slots_shape (T: Type) (n: usize) (v: vec (List_t T)) (fuel: na
     | Fail_ Failure => False
     end.
 Proof.
+
 remember (usize_to_nat n) as N.
 revert n HeqN fuel v.
-induction N ; intros.
+induction N; intros.
+
+(* TODO: Correct siphon_fuel
+revert fuel v;
+induction_usize_to_nat n as N; intros;
+siphon_fuel fuel;
+destruct_eqb n (0%usize) as Hn0.
+*)
 
 (* zero case *)
 1: {
 (* TODO: Coq unfolds the recursive def a second time with "destruct fuel" *)
+(* TODO: Tag fuel so a tactic can take care of it *)
 unfold hash_map_allocate_slots_fwd.
-destruct fuel. trivial.
+destruct fuel. 1: trivial.
 fold hash_map_allocate_slots_fwd.
 
 apply (f_equal Z.of_nat) in HeqN.
 rewrite usize_nat_to_Z in HeqN.
 simpl in HeqN.
 
-unfold scalar_eqb.
 simpl (to_Z 0 %usize).
-
 remember (to_Z n =? 0) as B.
-induction B ; apply eq_sym in HeqB.
- - now rewrite app_nil_r.
- - lia.
+induction B ; apply eq_sym in HeqB ; simpl.
+- now rewrite app_nil_r. (* can use "autorewrite with list" *)
+- exfalso. lia.
 }
 
 (* successor case *)
 1: {
 (* TODO: How to factorize repetitions properly in both cases ? *)
 unfold hash_map_allocate_slots_fwd.
-destruct fuel. trivial.
+destruct fuel. 1: trivial.
 fold hash_map_allocate_slots_fwd.
 
 (* Should be factorized with an induction tactic (same for the zero case). *)
-assert (H_SN := HeqN).
 apply (f_equal Z.of_nat) in HeqN.
 rewrite usize_nat_to_Z in HeqN.
 simpl in HeqN.
 
-unfold scalar_eqb.
 simpl (to_Z 0 %usize).
 
 remember (to_Z n =? 0) as B.
 induction B ; apply eq_sym in HeqB.
-1: { lia. }
+1: { exfalso. lia. }
 
-(* Annoying variable renaming then unfolding *)
-set (v2 := @ListNil T).
-rewrite_vec_push_back v v2 as "w"%string.
-unfold v2 in *.
+rewrite_vec_push_back v (@ListNil T) as w.
 
-rewrite_scalar_sub n (1%usize) as "y"%string.
+rewrite_scalar_sub n (1%usize) as y.
 
 simpl in Hy |- *.
 
 assert (P3: ((slots_to_chains v) ++ [[]]: list (chain_t T)) = slots_to_chains w).
 1: {
-  change ([[]]) with (map (@list_t_to_chain T) [ListNil]).
+  change ([[]]) with (map (@to_chain T) [ListNil]).
   unfold slots_to_chains.
   rewrite <-map_app.
   now rewrite <-Hw.
@@ -179,35 +244,95 @@ apply hm_allocate_slots_shape.
 apply (S_scalar_bounds n).
 Qed.
 
-(* Hashmap length *)
-
-Definition hm_length {T} (hm: Hash_map_t T) : usize :=
-  hm.(Hash_map_num_entries).
-
-Lemma hm_len_success {T} hm :
-  hash_map_len_fwd T hm = Return (hm_length hm).
+Lemma hm_allocate_slots_fuel (T: Type) (n: usize) (v: vec (List_t T)) (fuel: nat) :
+  vec_length v + to_Z n < usize_max ->
+  Z.of_nat fuel < to_Z n ->
+  hash_map_allocate_slots_fwd T fuel v n = Fail_ OutOfFuel.
 Proof.
-reflexivity.
+revert n v.
+induction fuel. 1: reflexivity.
+intros.
+
+unfold hash_map_allocate_slots_fwd.
+fold hash_map_allocate_slots_fwd.
+
+simpl (to_Z 0%usize).
+remember (to_Z n =? 0) as B.
+induction B ; apply eq_sym in HeqB.
+1: { lia. }
+
+rewrite_vec_push_back v (@ListNil T) as "w"%string.
+
+rewrite_scalar_sub n (1%usize) as "m"%string.
+simpl in Hm.
+
+apply (IHfuel m w). 2: lia.
+
+assert (vec_length w = vec_length v + 1). 2: lia.
+
+unfold vec_length.
+rewrite Hw.
+rewrite app_length.
+simpl.
+lia.
 Qed.
 
-(* Main invariants *)
+Lemma hm_allocate_slots_fail (T: Type) (n: usize) (v: vec (List_t T)) (fuel: nat) :
+    vec_length v + to_Z n > usize_max ->
+    Z.of_nat fuel >= to_Z n ->
+    hash_map_allocate_slots_fwd T fuel v n = Fail_ Failure.
+Proof.
+remember (usize_to_nat n) as N.
+revert n HeqN fuel v.
+induction N ; intros.
 
-Notation "x <-- c1 ; c2" := (result_prop_bind c1 (fun x => c2))
-(at level 61, c1 at next level, right associativity).
+(* Zero case *)
+1: {
+apply (f_equal Z.of_nat) in HeqN.
+rewrite usize_nat_to_Z in HeqN.
+simpl in HeqN.
 
-Definition key_is_in_hash_slot {T} (hm: Hash_map_t T) (i: slot_id) (j: chain_id) : Prop :=
-    kv <-- get_kv hm i j;
-    p  <-- get_hash_pos hm (fst kv);
-    (p = i).
+assert (vb := vec_len_in_usize v).
+lia.
+}
 
-Definition no_key_duplicate {T} (hm: Hash_map_t T) (i: slot_id) (j1 j2: chain_id) (p: j1 <> j2) : Prop :=
-    kv1 <-- get_kv hm i j1;
-    kv2 <-- get_kv hm i j2;
-    (fst kv1 <> fst kv2).
+(* Successor case *)
+1: {
+apply (f_equal Z.of_nat) in HeqN.
+rewrite usize_nat_to_Z in HeqN.
 
-Definition hm_invariants {T} (hm: Hash_map_t T) :=
-    (∀i j, key_is_in_hash_slot hm i j) /\
-    (∀i j1 j2 p, no_key_duplicate hm i j1 j2 p).
+unfold hash_map_allocate_slots_fwd.
+destruct fuel. 1: lia.
+fold hash_map_allocate_slots_fwd.
+
+simpl (to_Z 0%usize).
+remember (to_Z n =? 0) as B.
+induction B ; apply eq_sym in HeqB.
+1: { lia. }
+
+remember (vec_push_back (List_t T) v ListNil) as W.
+destruct W ; apply eq_sym in HeqW.
+2: { destruct e.
+- reflexivity.
+- exfalso. apply (vec_push_back_fuel _ _ HeqW).
+}
+rewrite res_bind_value.
+
+remember (usize_sub n 1%usize) as M.
+destruct M ; apply eq_sym in HeqM.
+2: { destruct e.
+- reflexivity.
+- exfalso. apply (scalar_sub_fuel _ _ HeqM).
+}
+rewrite res_bind_value.
+rewrite res_bind_id.
+
+apply IHN.
+- admit. (* exploit HeqM *)
+- admit. (* exploit HeqW *)
+- admit. (* exploit HeqM *)
+}
+Admitted.
 
 (* New hashmap *)
 
@@ -226,44 +351,158 @@ Lemma hm_new_success T fuel capacity max_load_dividend max_load_divisor :
   end.
 Proof.
 intro bounds.
-
 unfold hash_map_new_with_capacity_fwd.
+
+assert (Hv: vec_length (vec_new (List_t T)) + to_Z capacity <= usize_max).
+1: {
+  simpl.
+  now rewrite (proj2 (S_scalar_bounds _)).
+}
+assert (Hslots := hm_allocate_slots_shape T capacity (vec_new _) fuel Hv).
+
 remember (hash_map_allocate_slots_fwd T fuel
 (vec_new _) capacity) as S.
-set (Hslots := hm_allocate_slots_shape T capacity (vec_new _) fuel).
-rewrite <-HeqS in Hslots.
-destruct S.
-2: {
-  simpl.
-  destruct e.
-  - admit.
-  - trivial.
-}
+
+destruct S. 2: exact Hslots.
 rewrite res_bind_value.
 
 rewrite_scalar_mul capacity max_load_dividend as "x"%string.
 
 rewrite_scalar_div x max_load_divisor as "y"%string.
-1: { admit. }
-1: { admit. }
+1: {
+  assert (H := Z_div_pos (to_Z x) (to_Z max_load_divisor)).
+  lia.
+}
+1: {
+  assert (H := Z_div_lt (to_Z x) (to_Z max_load_divisor)).
+  lia.
+}
 
-split.
-2: { now unfold hm_length. }
+(* Why do we need the subsequent change ? *)
+set (hm := {|
+Hash_map_num_entries := 0 %usize;
+Hash_map_max_load_factor := (max_load_dividend, max_load_divisor);
+Hash_map_max_load := y;
+Hash_map_slots := v
+|}).
+change ({|
+Hash_map_num_entries := 0 %usize;
+Hash_map_max_load_factor := (max_load_dividend, max_load_divisor);
+Hash_map_max_load := y;
+Hash_map_slots := v
+|}) with hm.
 
-(* Invariants *)
-unfold hm_invariants.
+(* Invariants are easy as long as slots are empty *)
+assert (G: ∀i, ∀j, get_kv hm i j = Fail_ Failure).
+1: {
+intros.
+unfold get_kv.
+simpl (Hash_map_slots hm).
+simpl in Hslots.
+rewrite Hslots.
 
-Admitted.
+remember ((usize_to_nat i) <? (usize_to_nat capacity))%nat as C.
+destruct C ; apply eq_sym in HeqC.
+- rewrite Nat.ltb_lt in HeqC.
+  rewrite nth_error_repeat. 2: exact HeqC.
+  destruct (usize_to_nat j) ; reflexivity.
+- rewrite Nat.ltb_ge in HeqC.
+  rewrite (proj2 (nth_error_None _ _)).
+  + reflexivity.
+  + now rewrite repeat_length.
+}
+
+(* The invariants *)
+split. 2: now unfold hm_length.
+split ; intros.
+- unfold key_is_in_hash_slot.
+  now rewrite G.
+- unfold no_key_duplicate.
+  now rewrite G.
+Qed.
 
 Example hm_new_no_fail T : ∃fuel,
   hm <- hash_map_new_fwd T fuel;
   Return tt = Return tt.
 Proof.
 exists (33%nat).
-(* The simplification is too costly,
-   but the reflexivity proof works.
-*)
+(* The simplification is too costly but the reflexivity proof works. *)
 now cbv.
+Qed.
+
+(* Insertion *)
+
+Lemma hm_insert_in_list_fwd_shape {T} fuel k v l :
+  match hash_map_insert_in_list_fwd T fuel k v l with
+  | Return b => Bool.Is_true b <->
+      get_chain_value (to_chain l) k = None
+  | Fail_ OutOfFuel => True
+  | Fail_ Failure => False
+  end.
+Proof.
+revert fuel k v.
+induction l ; intros.
+2: { (* Nil case *)
+  unfold hash_map_insert_in_list_fwd.
+  destruct fuel ; intuition.
+}
+
+unfold hash_map_insert_in_list_fwd.
+destruct fuel. 1: trivial.
+fold hash_map_insert_in_list_fwd.
+
+(* scalar_eqb should be a Notation *)
+remember (s s= k) as B.
+rewrite Zeqb_sym in HeqB.
+destruct B ; apply eq_sym in HeqB.
+- split. 1: intuition.
+  intro H.
+  unfold to_chain, get_chain_value in H.
+  rewrite HeqB in H.
+  inversion H.
+- rewrite res_bind_id.
+  simpl.
+  rewrite HeqB.
+  apply IHl.
+Qed.
+
+Lemma hm_insert_in_list_back_shape {T} fuel k v l :
+  match hash_map_insert_in_list_back T fuel k v l with
+  | Return l' => match get_chain_value (to_chain l) k with
+    | None   => to_chain l' = (to_chain l) ++ [(k, v)]
+    | Some _ => to_chain l' = update_chain (to_chain l) k v
+  end
+  | Fail_ OutOfFuel => True
+  | Fail_ Failure => False
+  end.
+Proof.
+revert fuel k v.
+induction l ; intros.
+2: { (* Nil case *)
+  unfold hash_map_insert_in_list_back, get_chain_value.
+  destruct fuel ; reflexivity.
+}
+
+unfold hash_map_insert_in_list_back.
+destruct fuel. 1: trivial.
+fold hash_map_insert_in_list_back.
+
+remember (s s= k) as B.
+destruct B ; apply eq_sym in HeqB.
+1: { (* Lots of small changes on B... *)
+simpl.
+rewrite Zeqb_sym, HeqB.
+rewrite Z.eqb_eq in HeqB.
+apply scalar_Z_inj in HeqB.
+now rewrite HeqB.
+}
+
+assert (H := IHl fuel k v).
+set (hm := hash_map_insert_in_list_back T fuel k v l) in *.
+destruct hm ; simpl. 2: auto.
+rewrite Zeqb_sym, HeqB.
+destruct (get_chain_value (to_chain l) k) ;
+f_equal ; apply H.
 Qed.
 
 End Hashmap_Properties.
